Stabilisation.thy
@@ -5,14 +5,14 @@ begin
 section \<open>Stabilisation\<close>
 
 (* strongest weaker stable predicate *) (* \<box>\<^sup>\<rightarrow> *)
-definition swstable_pred
+definition swstable
   :: \<open>('a \<Rightarrow> bool) \<Rightarrow> ('a \<Rightarrow> 'a \<Rightarrow> bool) \<Rightarrow> ('a \<Rightarrow> bool)\<close>
   ("\<lfloor> _ \<rfloor>\<^bsub>_\<^esub>" [0,0] 90)
   where
   \<open>\<lfloor> P \<rfloor>\<^bsub>R\<^esub> \<equiv> \<lambda>s. \<forall>s'. R\<^sup>*\<^sup>* s s' \<longrightarrow> P s'\<close>
 
 (* weakest stronger stable predicate *) (* \<diamondsuit>\<^sup>\<leftarrow> *)
-definition wsstable_pred
+definition wsstable
   :: \<open>('a \<Rightarrow> bool) \<Rightarrow> ('a \<Rightarrow> 'a \<Rightarrow> bool) \<Rightarrow> ('a \<Rightarrow> bool)\<close>
   ("\<lceil> _ \<rceil>\<^bsub>_\<^esub>" [0,0] 90)
   where
@@ -21,41 +21,56 @@ definition wsstable_pred
 subsection \<open>basic logical properties\<close>
 
 lemma swstable_weaker: \<open>\<lfloor> P \<rfloor>\<^bsub>R\<^esub> \<le> P\<close>
-  by (force simp add: swstable_pred_def)
+  by (force simp add: swstable_def)
 
 lemma wsstable_stronger: \<open>P \<le> \<lceil> P \<rceil>\<^bsub>R\<^esub>\<close>
-  by (force simp add: wsstable_pred_def)
+  by (force simp add: wsstable_def)
+
+lemma wsstable_weaker_iff_swstable_stronger:
+  \<open>p \<le> \<lfloor> p \<rfloor>\<^bsub>R\<^esub> \<longleftrightarrow> \<lceil> p \<rceil>\<^bsub>R\<^esub> \<le> p\<close>
+  by (force simp add: wsstable_def swstable_def le_fun_def)
+
+definition stable :: \<open>('a \<Rightarrow> 'a \<Rightarrow> bool) \<Rightarrow> ('a \<Rightarrow> bool) \<Rightarrow> bool\<close> where
+  \<open>stable R p \<equiv> \<lfloor> p \<rfloor>\<^bsub>R\<^esub> = p\<close>
+
+lemma stable_iff:
+  \<open>stable R p \<longleftrightarrow> p \<le> \<lfloor> p \<rfloor>\<^bsub>R\<^esub>\<close>
+  by (simp add: stable_def antisym swstable_weaker)
+
+lemma stable_iff2:
+  \<open>stable R p \<longleftrightarrow> \<lceil> p \<rceil>\<^bsub>R\<^esub> \<le> p\<close>
+  by (simp add: stable_iff wsstable_weaker_iff_swstable_stronger)
 
 subsection \<open>(semi)distributivity properties\<close>
 
 lemma swstable_conj_distrib: \<open>\<lfloor> P \<sqinter> Q \<rfloor>\<^bsub>R\<^esub> = \<lfloor> P \<rfloor>\<^bsub>R\<^esub> \<sqinter> \<lfloor> Q \<rfloor>\<^bsub>R\<^esub>\<close>
-  by (force simp add: swstable_pred_def)
+  by (force simp add: swstable_def)
 
 lemma swstable_disj_semidistrib: \<open>\<lfloor> P \<rfloor>\<^bsub>R\<^esub> \<squnion> \<lfloor> Q \<rfloor>\<^bsub>R\<^esub> \<le> \<lfloor> P \<squnion> Q \<rfloor>\<^bsub>R\<^esub>\<close>
-  by (force simp add: swstable_pred_def)
+  by (force simp add: swstable_def)
 
 lemma wsstable_disj_distrib: \<open>\<lceil> P \<squnion> Q \<rceil>\<^bsub>R\<^esub> = \<lceil> P \<rceil>\<^bsub>R\<^esub> \<squnion> \<lceil> Q \<rceil>\<^bsub>R\<^esub>\<close>
-  by (force simp add: wsstable_pred_def)
+  by (force simp add: wsstable_def)
 
 lemma wsstable_conj_semidistrib: \<open>\<lceil> P \<sqinter> Q \<rceil>\<^bsub>R\<^esub> \<le> \<lceil> P \<rceil>\<^bsub>R\<^esub> \<sqinter> \<lceil> Q \<rceil>\<^bsub>R\<^esub>\<close>
-  by (force simp add: wsstable_pred_def)
+  by (force simp add: wsstable_def)
 
 subsection \<open>Rely Monotonicity\<close>
 
 lemma swstable_rely_antimono: \<open>R \<le> S \<Longrightarrow> \<lfloor> P \<rfloor>\<^bsub>S\<^esub> \<le> \<lfloor> P \<rfloor>\<^bsub>R\<^esub>\<close>
   using mono_rtranclp
-  by (force simp add: swstable_pred_def le_fun_def)
+  by (force simp add: swstable_def le_fun_def)
 
 lemma wsstable_rely_mono: \<open>R \<le> S \<Longrightarrow> \<lceil> P \<rceil>\<^bsub>R\<^esub> \<le> \<lceil> P \<rceil>\<^bsub>S\<^esub>\<close>
   using mono_rtranclp
-  by (force simp add: wsstable_pred_def le_fun_def)
+  by (force simp add: wsstable_def le_fun_def)
 
 subsection \<open>nested stabilisation\<close>
 
 lemma wsstable_absorb[simp]:
   assumes \<open>R\<^sup>*\<^sup>* = Ra\<^sup>*\<^sup>* OO Rb\<^sup>*\<^sup>*\<close>
   shows \<open>\<lceil> \<lceil> P \<rceil>\<^bsub>Ra\<^esub> \<rceil>\<^bsub>Rb\<^esub> = \<lceil> P \<rceil>\<^bsub>R\<^esub>\<close>
-  by (force simp add: assms wsstable_pred_def relcompp_apply fun_eq_iff)
+  by (force simp add: assms wsstable_def relcompp_apply fun_eq_iff)
 
 lemma wsstable_absorb1[simp]: \<open>R \<le> R' \<Longrightarrow> \<lceil> \<lceil> P \<rceil>\<^bsub>R\<^esub> \<rceil>\<^bsub>R'\<^esub> = \<lceil> P \<rceil>\<^bsub>R'\<^esub>\<close>
   by (simp add: rel_le_rtranscp_relcompp_absorb)
@@ -65,7 +80,7 @@ lemma wsstable_absorb2[simp]: \<open>R \<le> R' \<Longrightarrow> \<lceil> \<lce
 
 lemma swstable_absorb[simp]:
   \<open>R\<^sup>*\<^sup>* = Rb\<^sup>*\<^sup>* OO Ra\<^sup>*\<^sup>* \<Longrightarrow> \<lfloor> \<lfloor> P \<rfloor>\<^bsub>Ra\<^esub> \<rfloor>\<^bsub>Rb\<^esub> = \<lfloor> P \<rfloor>\<^bsub>R\<^esub>\<close>
-  by (force simp add: swstable_pred_def relcompp_apply imp_ex imp_conjL fun_eq_iff)
+  by (force simp add: swstable_def relcompp_apply imp_ex imp_conjL fun_eq_iff)
 
 lemma swstable_absorb1[simp]: \<open>R \<le> R' \<Longrightarrow> \<lfloor> \<lfloor> P \<rfloor>\<^bsub>R\<^esub> \<rfloor>\<^bsub>R'\<^esub> = \<lfloor> P \<rfloor>\<^bsub>R'\<^esub>\<close>
   by (simp add: rel_le_rtranscp_relcompp_absorb)
@@ -75,11 +90,11 @@ lemma swstable_absorb2[simp]: \<open>R \<le> R' \<Longrightarrow> \<lfloor> \<lf
 
 
 lemma wsstable_swstable_absorb[simp]: \<open>R \<le> R' \<Longrightarrow> \<lceil> \<lfloor> P \<rfloor>\<^bsub>R'\<^esub> \<rceil>\<^bsub>R\<^esub> = \<lfloor> P \<rfloor>\<^bsub>R'\<^esub>\<close>
-  unfolding wsstable_pred_def swstable_pred_def
+  unfolding wsstable_def swstable_def
   by (metis (opaque_lifting) predicate2D rtranclp.rtrancl_refl rtranclp_trans rtranclp_mono)
 
 lemma swstable_wsstable_absorb[simp]: \<open>R \<le> R' \<Longrightarrow> \<lfloor> \<lceil> P \<rceil>\<^bsub>R'\<^esub> \<rfloor>\<^bsub>R\<^esub> = \<lceil> P \<rceil>\<^bsub>R'\<^esub>\<close>
-  unfolding wsstable_pred_def swstable_pred_def
+  unfolding wsstable_def swstable_def
   by (metis (opaque_lifting) predicate2D rtranclp.rtrancl_refl rtranclp_trans rtranclp_mono)
 
 
@@ -93,7 +108,7 @@ lemma swstable_sepconj_semidistrib:
         \<exists>b1 b2. b1 ## b2 \<and> b = b1 + b2 \<and> R\<^sup>*\<^sup>* a1 b1 \<and> R\<^sup>*\<^sup>* a2 b2\<close>
   shows \<open>\<lfloor> P \<rfloor>\<^bsub>R\<^esub> \<^emph> \<lfloor> Q \<rfloor>\<^bsub>R\<^esub> \<le> \<lfloor> P \<^emph> Q \<rfloor>\<^bsub>R\<^esub>\<close>
   using rely_additivity_of_update
-  by (simp add: swstable_pred_def sepconj_def le_fun_def, metis)
+  by (simp add: swstable_def sepconj_def le_fun_def, metis)
 
 lemma wsstable_sepconj_semidistrib:
   fixes P Q :: \<open>'a \<Rightarrow> bool\<close>
@@ -101,7 +116,7 @@ lemma wsstable_sepconj_semidistrib:
     \<open>\<And>a1 a2 b. a1 ## a2 \<Longrightarrow> R\<^sup>*\<^sup>* (a1 + a2) b \<Longrightarrow> \<exists>b1 b2. b1 ## b2 \<and> b = b1 + b2 \<and> R\<^sup>*\<^sup>* a1 b1 \<and> R\<^sup>*\<^sup>* a2 b2\<close>
   shows \<open>\<lceil> P \<^emph> Q \<rceil>\<^bsub>R\<^esub> \<le> \<lceil> P \<rceil>\<^bsub>R\<^esub> \<^emph> \<lceil> Q \<rceil>\<^bsub>R\<^esub>\<close>
   using rely_additivity_of_update
-  by (simp add: wsstable_pred_def sepconj_def le_fun_def, metis)
+  by (simp add: wsstable_def sepconj_def le_fun_def, metis)
 
 end
 
@@ -229,7 +244,7 @@ lemma swstable_impl_distrib: \<open>\<box>(P \<leadsto> Q) \<sqinter> \<box> P \
 
 lemma wsstabledual_necessitation: \<open>\<top> \<le> P \<Longrightarrow> \<top> \<le> - (\<diamond>\<^sup>- (- P))\<close>
   by (metis (mono_tags, lifting) double_compl order_antisym predicate1I top_apply uminus_apply
-      wsstable_pred_def wsstable_stronger)
+      wsstable_def wsstable_stronger)
 
 lemma wsstabledual_impl_distrib: \<open>\<diamond>\<^sup>- Q \<le> \<diamond>\<^sup>-(-P \<sqinter> Q) \<squnion> \<diamond>\<^sup>-(P)\<close>
   by (metis (mono_tags, lifting) boolean_algebra.de_Morgan_disj double_compl inf.absorb1 inf_idem
